rewrite rule

pulse/examples/dsls/mini_steel/Pulse.Soundness.Common.fst
@@ -238,10 +238,6 @@ let frame_type (u:R.universe) =
 
 (** Type of sub_stt **)
 
-let stt_vprop_equiv_fv = R.pack_fv (mk_steel_wrapper_lid "vprop_equiv")
-let stt_vprop_equiv_tm = R.pack_ln (R.Tv_FVar stt_vprop_equiv_fv)
-let stt_vprop_equiv (t1 t2:R.term) = R.mk_app stt_vprop_equiv_tm [(t1, R.Q_Explicit); (t2, R.Q_Explicit)]
-
 let stt_vprop_post_equiv_fv = R.pack_fv (mk_steel_wrapper_lid "vprop_post_equiv")
 let stt_vprop_post_equiv_univ_inst u = R.pack_ln (R.Tv_UInst stt_vprop_post_equiv_fv [u])
 let stt_vprop_post_equiv (u:R.universe) (t t1 t2:R.term) = 
