pulse/examples/dsls/mini_steel/Pulse.Typing.fst
@@ -422,7 +422,15 @@ let comp_par (cL:comp{C_ST? cL}) (cR:comp{C_ST? cR}) (x:var) : comp =
     pre = Tm_Star (comp_pre cL) (comp_pre cR);
     post
   }
-  
+
+let comp_rewrite (p q:vprop) : comp =
+  C_STGhost Tm_EmpInames {
+			u = U_zero;
+			res = tm_unit;
+			pre = p;
+			post = q;
+		}
+
 let comp_admit (c:ctag) (s:st_comp) : comp =
   match c with
   | STT -> C_ST s
@@ -729,6 +737,14 @@ and st_typing (f:RT.fstar_top_env) : env -> st_term -> comp -> Type =
       st_typing f g eR cR ->
       st_typing f g (Tm_Par Tm_Unknown eL Tm_Unknown Tm_Unknown eR Tm_Unknown)
                     (comp_par cL cR x)
+
+  | T_Rewrite:
+		    g:env ->
+						p:vprop ->
+						q:vprop ->
+						tot_typing f g p Tm_VProp ->
+						vprop_equiv f g p q ->
+      st_typing f g (Tm_Rewrite p q) (comp_rewrite p q)
 
   | T_Admit:
       g:env ->
